mc_reify/get_set_reif.v
@@ -2,8 +2,6 @@ Require Import  Coq.Numbers.BinNums.
 Require Import compcert.lib.Maps.
 Require Import mc_reify.func_defs.
 
-Definition DEAD : expr typ func := Inj (typ:=typ) (inr (Other fFalse)).
-
 Definition as_tree (e : expr typ func) : option
   ((typ * expr typ func * expr typ func * expr typ func) + typ) := 
 match e with
@@ -14,33 +12,33 @@ match e with
   | _ => None
 end.
 
-Fixpoint set_reif (i : positive) (v : expr typ func) (m : expr typ func) :  expr typ func :=
+Fixpoint set_reif (i : positive) (v : expr typ func) (m : expr typ func) (ty : typ) :  expr typ func :=
 match (as_tree m) with
   | Some (inl (t,l,o,r)) (* Node l o r *)=>
     match i with 
       | xH => node l (some_reif v t) r t
-      | xO ii => node (set_reif ii v l) o r t
-      | xI ii => node l o (set_reif ii v r) t
+      | xO ii => node (set_reif ii v l ty) o r t
+      | xI ii => node l o (set_reif ii v r ty) t
     end
   | Some (inr t) => 
     match i with
       | xH => node (leaf t) (some_reif v t) (leaf t) t
-      | xO ii => node (set_reif ii v (leaf t)) (none_reif t) (leaf t) t
-      | xI ii => node (leaf t) (none_reif t) (set_reif ii v (leaf t)) t
+      | xO ii => node (set_reif ii v (leaf t) ty) (none_reif t) (leaf t) t
+      | xI ii => node (leaf t) (none_reif t) (set_reif ii v (leaf t) ty) t
     end
-  | _ => DEAD
+  | _ => (App (App (Inj (inr (Data (fset ty i)))) v) m)
 end.
 
 
-Fixpoint get_reif (i : positive) (m : expr typ func) :  expr typ func :=
+Fixpoint get_reif (i : positive) (m : expr typ func) ty :  expr typ func :=
 match (as_tree m) with
   | Some (inl (t,l,o,r)) (* Node l o r *)=>
     match i with 
       | xH => some_reif o t
-      | xO ii => get_reif ii l 
-      | xI ii => get_reif ii r 
+      | xO ii => get_reif ii l ty 
+      | xI ii => get_reif ii r ty 
     end
   | Some (inr t) => none_reif t
-  | _ => DEAD
+  | _ => (App (Inj (inr (Data (fget ty i))))  m)
 end.
 
