mc_reify/symexe_soundness.v
@@ -1,6 +1,42 @@
+Require Import floyd.proofauto.
+Require Import MirrorCore.RTac.Repeat.
+Require Import MirrorCore.RTac.Then.
+Require Import MirrorCore.RTac.Try.
+Require Import MirrorCore.RTac.First.
+Require Import MirrorCore.RTac.Fail.
+Require Import MirrorCore.RTac.Simplify.
 Require Import mc_reify.symexe.
+Require Import MirrorCore.RTac.RTac.
+Require Import mc_reify.types.
+Require Import mc_reify.funcs.
+Require Import mc_reify.func_defs.
+Locate THEN.
 
-Lemma THEN_sound : forall t1 t2 tbl,
+
+Section tbled.
+
+Parameter tbl : SymEnv.functions RType_typ.
+
+Let RSym_sym := RSym_sym tbl.
+Existing Instance RSym_sym.
+
+
+Let Expr_expr_fs := Expr_expr_fs tbl.
+Existing Instance Expr_expr_fs.
+
+Let Expr_ok_fs := Expr_ok_fs tbl.
+Existing Instance Expr_ok_fs.
+
+Let ExprVar_expr := @ExprVariables.ExprVar_expr.
+Existing Instance ExprVar_expr.
+
+Existing Instance MA.
+SearchAbout MentionsAnyOk.
+
+Instance MentionsAnyOk : MentionsAnyOk MA _ _.
+Admitted.
+
+Lemma THEN_sound : forall t1 t2,
 rtac_sound (Expr_expr := func_defs.Expr_expr_fs tbl) t1 -> rtac_sound (Expr_expr := func_defs.Expr_expr_fs tbl) t2 -> rtac_sound (Expr_expr := func_defs.Expr_expr_fs tbl) (THEN t1 t2). 
 intros. unfold THEN.
 unfold THEN'. 
@@ -11,8 +47,31 @@ apply INSTANTIATE_sound.
 apply runOnGoals_sound. auto.
 Qed.
 
+Definition APPLY_sound := (@APPLY_sound _ (expr typ func) _ _ _ _ _ _ _ _ _ _ _ _ (fun (subst : Type)
+                                 (SS : Subst subst (expr typ func))
+                                 (SU : SubstUpdate subst (expr typ func))
+                                 (tus tvs : tenv typ) 
+                                 (n : nat) (l r : expr typ func) 
+                                 (t3 : typ) (s1 : subst) =>
+                               @ExprUnify_simul.exprUnify subst typ func
+                                 RType_typ (func_defs.RSym_sym symexe.tbl)
+                                 Typ2_tyArr SS SU
+                                 (S (S (S (S (S (S (S (S (S (S O))))))))))
+                                 tus tvs n l r t3 s1) (ExprLift.vars_to_uvars_exprD')).
 
-Lemma SYMEXE_STEP_SOUND : forall tbl, rtac_sound (Expr_expr := func_defs.Expr_expr_fs tbl) (SYMEXE_STEP tbl).
+Definition EAPPLY_sound := (@EAPPLY_sound _ (expr typ func) _ _ _ _ _ _ _ _ _ _ _ _ (fun (subst : Type)
+                                 (SS : Subst subst (expr typ func))
+                                 (SU : SubstUpdate subst (expr typ func))
+                                 (tus tvs : tenv typ) 
+                                 (n : nat) (l r : expr typ func) 
+                                 (t3 : typ) (s1 : subst) =>
+                               @ExprUnify_simul.exprUnify subst typ func
+                                 RType_typ (func_defs.RSym_sym symexe.tbl)
+                                 Typ2_tyArr SS SU
+                                 (S (S (S (S (S (S (S (S (S (S O))))))))))
+                                 tus tvs n l r t3 s1) (ExprLift.vars_to_uvars_exprD')).
+
+Lemma SYMEXE_STEP_SOUND : rtac_sound (Expr_expr := func_defs.Expr_expr_fs tbl) (SYMEXE_STEP).
 intros. eapply AT_GOAL_sound.
 intros. destruct (get_delta_statement e);
 repeat match goal with
@@ -20,28 +79,100 @@ repeat match goal with
            destruct X; try apply FAIL_sound
        end.
 + unfold APPLY_SKIP.
-  generalize APPLY_sound.
-
-; eauto with typeclass_instances.
-  - apply ExprLift.vars_to_uvars_exprD'.
-  - intros. 
-    generalize (@exprUnify_sound subst typ func (RType_typ) _ (func_defs.RSym_sym tbl) _ _ _ _ _ _ _ 10).
-    unfold ExprUnify_common.unify_sound, ExprUnify_common.unify_sound_ind, LemmaApply.unify_sound.
- admit.
+  apply APPLY_sound. 
+  admit.
   - unfold skip_lemma. 
-    unfold lemmaD. simpl. intros. 
+    unfold Lemma.lemmaD. simpl. intros. 
     unfold ExprDsimul.ExprDenote.exprT_App.
     simpl.
     unfold exprT_Inj. apply semax_skip.
 + apply THEN_sound.
   - unfold APPLY_SET'.
     apply EAPPLY_sound; eauto with typeclass_instances.
-      * apply ExprLift.vars_to_uvars_exprD'.
       * admit.
-      * admit. (*red. simpl.
-        unfold lemmaD'. simpl.
-        unfold exprD'_typ0. simpl. unfold ExprDsimul.ExprDenote.exprD'.
-        simpl. simpl. *)
+      * Print set_lemma. unfold Lemma.lemmaD, set_lemma. unfold split_env.
+        unfold Lemma.lemmaD'.
+        Require Import MirrorCore.Util.ListMapT.
+        unfold Lemma.vars, Lemma.premises, Lemma.concl.
+        do 3 rewrite list_mapT_cons.
+        simpl exprD'_typ0. simpl.
+        Lemma exprD'_App_R_rw
+        : forall tus tvs td t e1 e2 e1D e2D,
+            typeof_expr tus tvs e2 = Some td ->
+            exprD' tus tvs td e2 = Some e2D ->
+            exprD' tus tvs (typ2 td t) e1 = Some e1D ->
+            exprD' tus tvs t (App e1 e2) = Some (exprT_App e1D e2D).
+        Proof.
+          admit.
+        Qed.
+        unfold exprD'_typ0, ExprI.exprD'. simpl. erewrite exprD'_App_R_rw.
+        2: reflexivity. 2: reflexivity.
+        Lemma exprD'_App_L_rw
+        : forall tus tvs td t e1 e2 e1D e2D,
+            typeof_expr tus tvs e1 = Some (typ2 td t) ->
+            exprD' tus tvs (typ2 td t) e1 = Some e1D ->
+            exprD' tus tvs td e2 = Some e2D ->
+            exprD' tus tvs t (App e1 e2) = Some (exprT_App e1D e2D).
+        Proof.
+          admit.
+        Qed.
+        Require Import get_set_reif_soundness.
+        2: eapply exprD'_App_L_rw; [ reflexivity | reflexivity | eapply set_reif_eq2 ].
+
+
+        Opaque Traversable.mapT HList.hlist_app Lemma.foralls.
+        simpl.
+
+        destruct ( @exprD'_typ0 typ (expr typ func) RType_typ Expr_expr_fs Prop
+                 Typ0_tyProp (@nil typ)
+                 (@cons typ (tyArr tyenviron tympred)
+                    (@cons typ (typtree tyfunspec)
+                       (@cons typ (tylist tympred)
+                          (@cons typ tyOracleKind
+                             (@cons typ (typtree (typrod tyc_type tyval))
+                                (@cons typ (typtree tyval)
+                                   (@cons typ tyval (@nil typ))))))))
+                 (@App typ func
+                    (@App typ func
+                       (@Inj typ func
+                          (@inr
+                             (sum
+                                (sum SymEnv.func
+                                   (ModularFunc.ILogicFunc.ilfunc typ))
+                                (BILogicFunc.bilfunc typ)) func'
+                             (Other (feq (tyoption tyval)))))
+                       (set_reif.rmsubst_eval_expr
+                          (@Var typ func (S (S (S (S (S O))))))
+                          (@Var typ func (S (S (S (S O))))) e0))
+                    (@App typ func
+                       (@Inj typ func
+                          (@inr
+                             (sum
+                                (sum SymEnv.func
+                                   (ModularFunc.ILogicFunc.ilfunc typ))
+                                (BILogicFunc.bilfunc typ)) func'
+                             (Other (fsome tyval))))
+                       (@Var typ func (S (S (S (S (S (S O)))))))))) eqn:?. simpl.
+
+destruct (exprD'_typ0 []
+                   [tyArr tyenviron tympred; typtree tyfunspec;
+                   tylist tympred; tyOracleKind;
+                   typtree (typrod tyc_type tyval); 
+                   typtree tyval; tyval]
+                   (App
+                      (App
+                         (Inj (inr (Other (feq (tyArr tyenviron tympred)))))
+                         (App
+                            (App
+                               (App (Inj (inr (Smx fassertD)))
+                                  (Inj (inr (Data (..)))))
+                               (App
+                                  (App (Inj (inr (..)))
+                                     (get_set_reif.set_reif i 
+                                        (Var 6%nat) 
+                                        (Var 5%nat))) 
+                                  (Var 4%nat))) (Var 2%nat))) 
+                      (Var 0%nat))).
   - 
         
 
